Mica/SourceTinyML.lean
@@ -6,6 +6,7 @@ import Mica.SourceTinyML.Untyped
 import Mica.SourceTinyML.Typed
 import Mica.SourceTinyML.Assertions
 import Mica.SourceTinyML.TypeConstraints
+import Mica.SourceTinyML.Unification
 import Mica.SourceTinyML.Typing
 import Mica.SourceTinyML.Printer
 import Mica.SourceTinyML.World
